Refactored HelpfulFunctions.v (split into Core.v and ListUtil.v).  Removed BitcoinMultiplication folder.

src/Arithmetic/Core.v
@@ -188,6 +188,47 @@ Module Associational.
     now rewrite eval_reduce_adjusted.
   Qed.
 
+  Definition split_one (s:Z) (w fw : Z) (p:list (Z*Z)) :=
+    let hi_lo := partition (fun t => (fst t =? w)) p in
+      (snd hi_lo, map (fun t => (fst t / fw, snd t)) (fst hi_lo)).
+
+  Lemma eval_split_one s w fw p (s_nz:s<>0) (fw_nz:fw<>0) (w_fw : w mod fw = 0) (fw_s : fw mod s = 0):
+    Associational.eval (fst (split_one s w fw p)) + fw * Associational.eval (snd (split_one s w fw p)) = Associational.eval p.
+  Proof.
+    remember (Z_div_exact_full_2 _ _ fw_nz w_fw) as H2.
+    clear HeqH2 fw_nz w_fw.
+    induction p as [|t p'].
+    - simpl. cbv [Associational.eval]. simpl. lia.
+    - cbv [split_one]. simpl. destruct (fst t =? w) eqn:E.
+      + simpl in IHp'. remember (partition (fun t0 : Z * Z => fst t0 =? w) p') as thing.
+        destruct thing as [thing1 thing2]. simpl. simpl in IHp'. repeat rewrite Associational.eval_cons.
+        ring_simplify. simpl.
+        apply Z.eqb_eq in E. rewrite E. rewrite <- H2. rewrite <- IHp'. ring.
+      + simpl in IHp'. remember (partition (fun t0 : Z * Z => fst t0 =? w) p') as thing.
+        destruct thing as [thing1 thing2]. simpl. simpl in IHp'. repeat rewrite Associational.eval_cons.
+        rewrite <- IHp'. ring.
+  Qed.
+
+  (*assumes that (H1 : w mod fw = 0) (H2 : fw mod s = 0) *)
+  Definition reduce_one (s:Z) (w fw : Z) (c: Z) (p:list _) : list (Z*Z) :=
+    let lo_hi := split_one s w fw p in
+    fst lo_hi ++ map (fun thing => (fst thing, snd thing * (c * (fw / s)))) (snd lo_hi).
+
+  Lemma eval_map_mul_snd (x:Z) (p:list (Z*Z))
+    : Associational.eval (List.map (fun t => (fst t, snd t * x)) p) = x * Associational.eval p.
+  Proof. induction p; push; nsatz. Qed.
+
+  Lemma eval_reduce_one s w fw c p (s_nz:s<>0) (fw_nz:fw<>0) (w_fw : w mod fw = 0) (fw_s : fw mod s = 0)
+                               (modulus_nz: s - c<>0) :
+              Associational.eval (reduce_one s w fw c p) mod (s - c) =
+              Associational.eval p mod (s - c).
+  Proof using Type.
+    cbv [reduce_one]; push.
+    rewrite eval_map_mul_snd. rewrite <- Z.mul_assoc.
+    rewrite <- (reduction_rule _ _ _ _ modulus_nz).
+    rewrite Z.mul_assoc. rewrite <- (Z_div_exact_full_2 fw s s_nz fw_s). rewrite eval_split_one; trivial.
+  Qed.
+
   (*
   Definition splitQ (s:Q) (p:list (Z*Z)) : list (Z*Z) * list (Z*Z)
     := let hi_lo := partition (fun t => (fst t * Zpos (Qden s)) mod (Qnum s) =? 0) p in
@@ -464,6 +505,59 @@ Module Associational.
       push; [|rewrite IHp]; reflexivity.
   Qed.
 
+  Definition value_at_weight (a : list (Z * Z)) (d : Z) :=
+    fold_right (fun p sum => if (d =? fst p) then (sum + snd p) else sum) 0 a.
+
+  Lemma value_at_weight_works a d : d * (value_at_weight a d) = Associational.eval (filter (fun p => d =? fst p) a).
+  Proof.
+    induction a as [| a0 a' IHa'].
+    - cbv [Associational.eval]. simpl. ring.
+    - simpl. destruct (d =? fst a0) eqn:E.
+      + rewrite Associational.eval_cons. rewrite <- IHa'. apply Z.eqb_eq in E. rewrite E. ring.
+      + apply IHa'.
+  Qed.
+
+  Definition firsts (a : list (Z*Z)) :=
+    map (fun p => fst p) a.
+
+  Lemma not_in_value_0 a d : ~ In d (firsts a) -> value_at_weight a d = 0.
+  Proof.
+    intros H. induction a as [| x a' IHa'].
+    - reflexivity.
+    - simpl. destruct (d =? fst x) eqn:E.
+      + exfalso. apply H. simpl. left. apply Z.eqb_eq in E. symmetry. apply E.
+      + apply IHa'. intros H'. apply H. simpl. right. apply H'.
+  Qed.
+
+  Definition dedup_weights a :=
+    map (fun d => (d, value_at_weight a d)) (just_once Z.eqb (firsts a)).
+
+  Lemma map_eq (x y : Z) l a : ~ In x l ->
+    map (fun d : Z => (d, value_at_weight a d)) l = map (fun d : Z => (d, if d =? x then (value_at_weight a d + y) else value_at_weight a d)) l.
+  Proof.
+    intros H. induction l as [|x' l' IHl'].
+    - reflexivity.
+    - simpl. destruct (x' =? x) eqn:E.
+      + exfalso. apply H. apply Z.eqb_eq in E. rewrite E. simpl. left. reflexivity.
+      + rewrite IHl'.
+        -- reflexivity.
+        -- intros H'. apply H. simpl. right. apply H'.
+  Qed.
+
+  Theorem eval_dedup_weights a : Associational.eval (dedup_weights a) = Associational.eval a.
+  Proof.
+    induction a as [| a0 a'].
+    - reflexivity.
+    - cbv [dedup_weights]. simpl. destruct (is_in Z.eqb (fst a0) (just_once Z.eqb (firsts a'))) eqn:E.
+      + apply (is_in_true_iff Z.eqb Z.eqb_eq) in E. rewrite <- (just_once_in_iff Z.eqb Z.eqb_eq) in E. apply (just_once_split Z.eqb Z.eqb_eq) in E.
+        destruct E as [l1 [l2 [H1 [H2 H3] ] ] ]. rewrite H1. repeat rewrite map_app. rewrite <- (map_eq _ _ _ _ H2).
+        rewrite <- (map_eq _ _ _ _ H3). repeat rewrite Associational.eval_app. simpl. rewrite Z.eqb_refl. repeat rewrite Associational.eval_cons.
+        rewrite <- IHa'. simpl. rewrite Associational.eval_nil. cbv [dedup_weights]. rewrite H1.
+        repeat rewrite map_app. repeat rewrite Associational.eval_app. cbv [Associational.eval]. simpl. ring.
+      + simpl. rewrite Z.eqb_refl. apply (is_in_false_iff Z.eqb Z.eqb_eq) in E. rewrite <- (map_eq _ _ _ _ E). repeat rewrite Associational.eval_cons.
+        simpl. rewrite <- IHa'. cbv [dedup_weights]. f_equal. f_equal. rewrite <- (just_once_in_iff Z.eqb Z.eqb_eq) in E. rewrite (not_in_value_0 _ _ E). ring.
+  Qed.
+
   Section Carries.
     Definition carryterm (w fw:Z) (t:Z * Z) :=
       if (Z.eqb (fst t) w)
@@ -489,6 +583,36 @@ Module Associational.
       eval (carry w fw p) = eval p.
     Proof using Type*. cbv [carry]; induction p; push; nsatz. Qed.
     Hint Rewrite eval_carry using auto : push_eval.
+
+  (* 'carrying down', aka borrowing *)
+  Definition carryterm_down (w fw:Z) (t:Z * Z) :=
+      let quot := w / fw in
+      if (Z.eqb (fst t) w)
+        then [(quot, snd t * fw)]
+        else [t].
+
+  Lemma eval_carryterm_down w fw (t:Z * Z) (fw_nz:fw<>0) (w_fw:w mod fw = 0) :
+        Associational.eval (carryterm_down w fw t) = Associational.eval [t].
+  Proof using Type*.
+    cbv [carryterm_down Let_In]; break_match; push; [|trivial].
+    pose proof (Z.div_mod (snd t) fw fw_nz).
+    rewrite Z.eqb_eq in *.
+    ring_simplify. rewrite Z.mul_comm. rewrite Z.mul_assoc. rewrite <- Z_div_exact_full_2; lia.
+  Qed.
+
+  Definition carry_down (w fw:Z) (p:list (Z*Z)) :=
+    flat_map (carryterm_down w fw) p.
+
+  Lemma eval_carry_down w fw p (fw_nz:fw<>0) (w_fw:w mod fw = 0):
+        Associational.eval (carry_down w fw p) = Associational.eval p.
+  Proof using Type*.
+    cbv [carry_down carryterm_down]. induction p.
+    - trivial.
+    - push. destruct (fst a =? w) eqn:E.
+      + rewrite Z.mul_comm. rewrite <- Z.mul_assoc. rewrite <- Z_div_exact_full_2; lia.
+      + rewrite IHp. lia.
+  Qed.
+
   End Carries.
 End Associational.
 
